Verif: semi-complete refinement proof for monitor delete operation

theories/Verif/refine.v
@@ -1,170 +1,254 @@
 From stdpp Require Import prelude.
 From compcert Require Import Integers.
+From RecordUpdate Require Import RecordUpdate.
 From S3K.Barocq Require Import S3K_ShallowR.
-From S3K.ExecSem Require Import kstate cap ctx exec util.
-From S3K.Verif Require Import repr aux.
+From S3K.ExecSem Require Import kstate cap ctx exec util config.
+From S3K.Verif Require Import repr barocq_aux tactics.
 From S3K.BarocqComp Require Import Option Barray Intop Utils.
 From S3K.BarocqComp Require Import ShallowNotations.
-From RecordUpdate Require Import RecordUpdate.
 
 Set Implicit Arguments.
 
-(* Mon_valid_access safe execution theorem,
-   with post condition, only one direction (b = true) is needed *)
-Theorem mon_valid_access_safe :
-  forall kb owner i,
-  exists b, Mon_valid_access kb owner i = Some b /\
-    (b = true -> (usize_to_nat i < length kb.(types_kstate_mon_table))%nat).
-Proof.
-  unfold Mon_valid_access.
-  intros.
-  case_match.
-  - solve_get.
-    + rewrite mon_table_len.
-      apply nat_lt_iff_int64_ltu.
-      assumption.
-    + by eexists.
-  - by eexists.
-Qed.
+(** * Refinement proofs *)
 
-(* TODO this is not helping
-Hint Resolve Rkstate_equiv : mon.
-Hint Resolve Rmon_equiv : mon.
- *)
+(** ** Refinement with safe execution *)
+Section SafeRefine.
 
-(* Mon_valid_access is correct with regard to cap_owner_get,
-   safe execution is implied. *)
-Theorem mon_valid_access_safe_correct :
-  forall kb ka ownera ownerb ia ib cap_opt,
-  Rkstate ka kb ->
-  Rpid ownera ownerb ->
-  Rnat ia ib ->
-  cap_owner_get ka.(kmon_tbl) ownera ia = cap_opt ->
-  Mon_valid_access kb ownerb ib =
-    Some (match cap_opt with
-          | Some _ => true
-          | None => false
-          end).
-Proof.
-  intros until 3.
-  unfold cap_owner_get, Mon_valid_access.
-  case_match. (* cap_get *)
-  - edestruct Rmon_table_bget as [vb [Hvb HRmonvb]]; eauto.
-    eapply Rkstate_equiv; eauto.
-    (* Need to get Int64.ltu ib Config_mon_table_size = false from Hvb,
-       more generally, a tactic that finds the first conditional in the
-       Barocq function and resolves its result from the hypotheses *)
-    replace (Int64.ltu ib Config_mon_table_size) with true; cycle 1.
-    { apply barray_get_Some_cond in Hvb. 
-      rewrite mon_table_len in Hvb.
-      symmetry; by apply nat_lt_iff_int64_ltu. }
-      rewrite Hvb; simpl.
-    case_decide. (* owner equal? *)
-    + intros.
-      subst.
-      f_equal.
-      replace (types_mon_t_owner vb) with ownerb.
-      apply Int64.eq_true.
-      { symmetry. eapply Rpid_opt_eq; eauto. apply Rmon_equiv. auto. }
-    + intros. subst. f_equal.
-      apply Int64.eq_false.
-      eapply Rpid_opt_neq; eauto. apply Rmon_equiv. auto.
-  - replace (Int64.ltu ib Config_mon_table_size) with false; cycle 1.
-    { admit. (* similar process as above *) }
-    intros.
-    f_equal.
-    by subst.
-Admitted.
+(** A: abstract type, B: concrete type *)
+Variable A B : Type.
 
-Theorem mon_delete_safe :
-  forall kb ownerb ib,
-  exists kb', Mon_delete kb ownerb ib = Some kb'.
-Proof.
-  unfold Mon_delete.
-  intros.
-  edestruct mon_valid_access_safe as [b [Hb Hva]].
-  rewrite Hb.
-  destruct b.
-  - specialize (Hva eq_refl).
-    solve_get.
-    solve_set.
-    by eexists.
-  - by eexists.
-Qed.
+(** R: Refinement mapping *)
+Variable R : A -> B -> Prop.
+
+(** Concrete code is safe while preserving refinement mapping. *)
+Definition safe_refine (a : A) (ob : option B) :=
+  exists b, ob = Some b /\ R a b.
+
+(** Concrete code is safe given that abstract code is safe, also maintaining
+refinement mapping. *)
+Definition safe_refine_opt (oa : option A) (ob : option B) :=
+  forall a, oa = Some a -> exists b, ob = Some b /\ R a b.
+
+Lemma safe_refine_opt_None : forall b, safe_refine_opt None b.
+Proof. done. Qed.
+
+Lemma safe_refine_opt_Some : forall a ob,
+  safe_refine a ob ->
+  safe_refine_opt (Some a) ob.
+Proof. unfold safe_refine_opt; intros; by inv H0. Qed.
+
+Lemma safe_refine_Some : forall a b,
+  R a b ->
+  safe_refine a (Some b).
+Proof. unfold safe_refine; intros; by exists b. Qed.
+
+End SafeRefine.
+
+(** ** Hints and tactics *)
+
+From Ltac2 Require Import Ltac2 Printf.
+
+Create HintDb s3k_unfold.
+(** Abstract helper functions to unfold *)
+Hint Unfold cap_get : s3k_unfold.
+Hint Unfold cap_owner_get : s3k_unfold.
+
+(** Barocq helper functions to unfold *)
+Hint Unfold Mon_valid_access : s3k_unfold.
+
+(** Hint database for backward reasoning about data correspondence between
+the abstract and concrete models. *)
+Create HintDb s3k_inv.
+
+Hint Resolve safe_refine_opt_None safe_refine_opt_Some safe_refine_Some : s3k_inv.
+Hint Resolve Rkstate_inv Rkstate_with_err_inv : s3k_inv.
+Hint Resolve Rmon_table_set Rmon_set_owner : s3k_inv.
+Hint Resolve Rmon_table_inv_Rkstate Rtsl_table_inv_Rkstate Rptable_inv_Rkstate : s3k_inv.
+
+Hint Extern 10 (Rpid_opt _ _) => reflexivity : s3k_inv.
+Hint Extern 10 (_ = _) => reflexivity : s3k_inv.
+Hint Extern 1 (Rmon_table _ _) => progress simpl : s3k_inv.
+Hint Extern 1 (Rtsl_table _ _) => progress simpl : s3k_inv.
+Hint Extern 1 (Rptable _ _) => progress simpl : s3k_inv.
+(** Replace CapTable l with canonical form *)
+Hint Extern 1 (Rmon_table (CapTable _) _) =>
+  match! goal with | [ h : _ = CapTable _ |- _ ] => let h := Control.hyp h in rewrite <- $h end.
 
 Opaque cap_set.
 
-Theorem mon_delete_corres :
-  forall ka kb ownera ownerb ia ib ka' kb' erra,
-  Rkstate ka kb ->
-  Rpid ownera ownerb ->
-  Rnat ia ib ->
-  exec_mon_delete ka ownera ia = (ka', erra) ->
-  Mon_delete kb ownerb ib = Some kb' ->
-  Rkstate_with_err (ka', erra) kb'.
-Proof.
-  unfold exec_mon_delete, Mon_delete.
-  intros until 3.
-  case_match. (* case analysis on result of cap_owner_get *)
-  - erewrite mon_valid_access_safe_correct by eauto.
-    simpl.
-    (* post conditions for cap_owner_get ... = Some x *)
-    edestruct cap_owner_get_Some; eauto.
-    (* consequences in Barocq of the above post conditions *)
-    edestruct Rmon_table_bget as [vb [Hvb HRmon]]; eauto.
-    { apply Rkstate_equiv; eauto. }
-    rewrite Hvb; simpl.
-    (* Barray set operation guaranteed to succeed *)
-    break_bind.
-    intros.
-    inv_all.
-    apply Rkstate_with_err_equiv.
-    split.
-    + apply Rkstate_equiv.
-      apply Rkstate_equiv in H.
-      simpl.
-      intuition.
-      eapply Rmon_table_bset; eauto.
-      apply set_owner_None_preserve_Rmon; auto.
-    + done.
-  - (* cap_owner_get = None *)
-    erewrite mon_valid_access_safe_correct by eauto.
-    simpl.
-    intros.
-    inv_all.
-    apply Rkstate_with_err_equiv.
-    split.
-    + done.
-    + admit. (* FIXME this is just because errcode is incorrect for now ... *)
-Admitted.
+Ltac2 fail_with_msg (s : string) := Control.backtrack_tactic_failure s.
 
-Theorem mon_delete_safe_corres :
-  forall ka kb ownera ownerb ia ib ka' erra,
-    Rkstate ka kb ->
-    Rpid ownera ownerb ->
-    Rnat ia ib ->
-    exec_mon_delete ka ownera ia = (ka', erra) ->
-    (exists kb', Mon_delete kb ownerb ib = Some kb' /\
-      Rkstate_with_err (ka', erra) kb').
+Ltac2 Notation "trivial_erewrite"
+  rw(list1(rewriting, ","))
+  cl(opt(clause))
+  tac(opt(seq("by", thunk(tactic)))) :=
+  unshelve (rewrite0 true rw cl tac); auto; Control.assert_true (Int.equal (Control.numgoals ()) 1).
+
+(** Solve R correspondence using backward reasoning *)
+Ltac2 solve_corres () :=
+  eauto 15 with s3k_inv.
+
+(* Try solve correspondence term t and return the hypothesis, may fail. *)
+Ltac2 get_or_solve_corres (t : constr) : constr :=
+  printf "solving %t" t;
+  let oh := List.find_opt (fun (_,_,ty) => Constr.equal t ty) (Control.hyps ()) in
+  match oh with
+  (* if in goal already *)
+  | Some (h_ident, _, _) => Control.hyp h_ident
+  (* try solve it if not *)
+  | None => 
+    let h := Fresh.in_goal @HR in
+    assert $t as $h by solve_corres () ; printf "solved"; Control.hyp h
+  end.
+
+(** Case analysis on whether an abstract capability is physically deleted or not. *)
+Ltac2 forward_abstract_opt_cap (t : constr) :=
+  destruct $t >
+  [ (* Some case, do nothing. *)
+    ()
+  |
+    (* None case *)
+    (* Since in principle a system call should never touch a physically deleted
+       capability, we can be sure that the concrete level must return invalid
+       access. This is ensured since Int64.eq vb.(types_mon_t_owner) owner is alway
+       false in this case. *)
+    erewrite Rmon_None_corres by eauto
+  ].
+
+About mon_lookup_Some_len.
+
+(* Forward reasoning on the result of abstract capability lookup,
+derive the corresponding conditions in the concrete model. *)
+Ltac2 forward_abstract_lookup (h : constr) :=
+  lazy_match! (Constr.type h) with
+  | ?ta !! ?ia = ?ova =>
+    (* find corresponding tb.[ib] in the concrete layer *)
+    lazy_match! goal with
+    | [ |- context[?tb.[USIZE.of_u64 ?ib]]] =>
+      (* try solve R ta tb and R ia ib *)
+      let htable := get_or_solve_corres '(Rmon_table (CapTable $ta) $tb) in
+      let hi := get_or_solve_corres '(Rnat $ia $ib) in
+      lazy_match! ova with
+      (* if abstract lookup returns Some *)
+      | Some ?va =>
+        let vb := Fresh.in_goal @vb in
+        let hvb := Fresh.in_goal @Hvb in
+        let hrmon := Fresh.in_goal @HRmon in
+        destruct (mon_get_Some_corres $htable $hi $h) as [$vb [$hvb $hrmon]];
+        printf "destructed";
+        let hvb:= Control.hyp hvb in
+        (* Rewrite the result of barocq get *)
+        trivial_erewrite ?($hvb), ?(mon_lookup_Some_len _ _ $h $hi); simpl;
+        (* destruct abstract optional capability *)
+        printf "Case analysis on whether abstract capability is physically deleted or not ";
+        Control.enter (fun _ => forward_abstract_opt_cap va)
+      (* if abstract lookup returns None *)
+      | None =>
+        (* If abstract model fails, holds vacuously.
+           Otherwise abstract model handles the lookup error, simplify in concrete. *)
+        trivial_erewrite ?(mon_lookup_None_len _ _ $h $hi); simpl; auto with s3k_inv
+      end
+    | [ |- _] => fail_with_msg "Found no correspondence for abstract lookup in concrete model."
+    end
+  end.
+
+(** Derive finer correspondence results from the hypotheses. *)
+Ltac2 forward_corres () :=
+  match! goal with
+  | [ h : Rmon (Some ?va) ?vb |- context[?vb] ] =>
+      apply Rmon_Some_corres in $h; ltac1:(h |- destruct_and? h) (Ltac1.of_ident h)
+  | [ h : Rnat ?va ?vb |- context[?vb] ] =>
+      unfold Rnat, fun_hrel in $h
+  | [ h1 : Rpid_opt ?ova ?vb,
+      h2 : Rpid_opt ?ova' ?vb' |- context[?vb] ] =>
+      let h1 := Control.hyp h1 in
+      let h2 := Control.hyp h2 in
+      rewrite (Rpid_opt_inj $h1 $h2) in *
+  end.
+
+(** Solve concrete condition. *)
+Ltac2 solve_concrete_cond () :=
+  printf "Trying to solve concrete condition: %t" (Control.goal ());
+  repeat (forward_corres ());
+  unfold int64_to_nat in *;
+  ltac1:(norm_cmp);
+  ltac1:(rep_lia).
+
+(** Find head concrete condition and try simplifying it. *)
+Ltac2 forward_concrete_cond () :=
+  match! goal with
+  | [ |- safe_refine _ _ (if ?b then _ else _)] =>
+    (* Try simplify the if branch *)
+    let hcond := Fresh.in_goal @Hcond in
+    first [
+      assert ($b = true) as $hcond by solve_concrete_cond () |
+      assert ($b = false) as $hcond by solve_concrete_cond () ];
+    let hcond := Control.hyp hcond in
+    rewrite! $hcond; simpl
+  | [ |- _ ] => printf "Failed to solve any concrete condition."
+  end.
+
+(** Reason Barocq set success and simplify. *)
+Ltac2 forward_concrete_map_set () :=
+  lazy_match! goal with
+  | [ h: ?tb.[?ib] = Some _ |- context[?tb.[?ib <- ?v]]] =>
+    (* Rewrite the result of barocq set at the same index *)
+    let h := Control.hyp h in
+    let tb' := Fresh.in_goal @tb in
+    let htb' := Fresh.in_goal @Htb in
+    destruct (bget_Some_bset_Some $tb $ib $v $h) as [$tb' $htb'];
+    let htb' := Control.hyp htb' in
+    rewrite $htb'; simpl
+  end.
+  
+(** Find decision in abstract model, do case analysis and try simplifying and
+synchronizing the concrete model. *)
+Ltac2 forward_abstract () :=
+  match! goal with
+  | [ |- context[match ?t with  _ => _ end ] ] =>
+      first [
+        lazy_match! (Constr.type t) with
+        (* Destruct cap table of single construtor CapTable *)
+        | mon_table_t => destruct $t eqn:?; printf "Getting rid of CapTable"
+        end |
+        (* Destruct result of table get *)
+        lazy_match! t with
+          ?l !! ?ia =>
+            let h := Fresh.in_goal @Hlookup in
+            printf "Case analysis on capability table lookup";
+            destruct $t eqn:$h; Control.enter (fun () => forward_abstract_lookup (Control.hyp h))
+        end |
+        (* Find decide P *)
+        ltac1:(case_decide); Control.enter (fun () => forward_concrete_cond () )
+      ]
+  end.
+
+
+(** ** Refinement proofs for capability operations. *)
+
+Section S3KRefine.
+
+Variable ka : kstate_t.
+Variable kb : Types_kstate.
+
+(** This should be evident from abstract kernel well-formedness, however
+since it's not ported yet use hypothesis for now. *)
+Hypothesis mon_table_size : ctable_size ka.(kmon_tbl) = MON_SZ.
+
+Theorem mon_delele_safe_refine :
+  forall ownera ownerb ia ib,
+  Rkstate ka kb ->
+  Rpid_opt (Some ownera) ownerb ->
+  Rnat ia ib ->
+  safe_refine Rkstate_with_err (exec_mon_delete ka ownera ia) (Mon_delete kb ownerb ib).
 Proof.
-  intros. 
-  edestruct mon_delete_safe as [kb' Hkb'].
-  rewrite Hkb'.
-  eexists.
-  split.
-  - reflexivity.
-  - eapply mon_delete_corres; eauto.
+  intros.
+  unfold exec_mon_delete, Mon_delete.
+  ltac1:(autounfold with s3k_unfold).
+  repeat (forward_abstract ()).
+  forward_concrete_map_set ().
+  all: solve_corres ().
 Qed.
 
-(* Alternatively, one can prove mon_delete_safe_corres in one shot *)
-Theorem mon_delete_safe_corres' :
-  forall ka kb ownera ownerb ia ib ka' erra,
-    Rkstate ka kb ->
-    Rpid ownera ownerb ->
-    Rnat ia ib ->
-    exec_mon_delete ka ownera ia = (ka', erra) ->
-    (exists kb', Mon_delete kb ownerb ib = Some kb' /\
-      Rkstate_with_err (ka', erra) kb').
-Proof.
-Admitted.
+End S3KRefine.
 
