theories/Verif/repr.v
@@ -1,27 +1,40 @@
 From stdpp Require Import prelude.
 From compcert Require Import Integers.
 From S3K.Barocq Require Import S3K_ShallowR.
-From S3K.ExecSem Require Import kstate cap ctx exec util proc sched.
-From S3K.BarocqComp Require Import Intop Option.
+From S3K.ExecSem Require Import kstate cap ctx exec util proc sched config.
+From S3K.BarocqComp Require Import Option Barray Intop Utils.
+From S3K.BarocqComp Require Import ShallowNotations.
+From S3K.Verif Require Import barocq_aux tactics.
+From RecordUpdate Require Import RecordUpdate.
 
 Import IntopNotations.
 
+Set Implicit Arguments.
+
+(** * Refinement mapping definitions. *)
+
+(** [a] [b] are related by total specification function [f]. *)
 Definition fun_hrel {A} {B} (f : B -> A) : A -> B -> Prop :=
   fun a b => f b = a.
 
+(** [a] [b] are related by partial specification function [f]. *)
 Definition ofun_hrel {A} {B} (f : B -> option A) : A -> B -> Prop :=
   fun a b => f b = Some a.
 
-Definition usize_to_nat (i : usize) : nat := Z.to_nat (USIZE.to_Z i).
-
+(** Int64 integer to abstract process ID. 0UL encodes empty PID. *)
 Definition int64_to_pid (i : int64) : option nat :=
-  if Int64.eq i 0UL then None else Some ((int64_to_nat i) - 1).
+  if Int64.eq i 0UL then None else Some ((int64_to_nat i) - 1)%nat.
 
+(** Partial mapping from capability fields to a capability slot (may be empty).
+Disallow the case where [cfree] is zero while [owner] is not [None].
+Essentially this is encoding one of the well-formedness properties, however
+it is necessary since otherwise concrete capability delete operation could physically
+delete a capability. *)
 Definition mk_cap_opt {A} (owner : option nat) (free size : nat) (data : A) : option (option (cap_t A)) :=
   match free with
   | O => match owner with
          | None => Some None (* physically deleted *)
-         | Some _ => None (* Invalid state, when owner exists, free must be greater than 0 *)
+         | Some _ => None (* Invalid state, when owner exists, cfree must be greater than 0 *)
          end
   | S _ => Some
              (Some {| cowner := owner;
@@ -30,6 +43,7 @@ Definition mk_cap_opt {A} (owner : option nat) (free size : nat) (data : A) : op
                       cdata := data; |})
   end.
 
+(** Mappings from concrete capability to abstract capability. *)
 Definition tsl_up (tsl : Types_tsl_t) : option (option (cap_t tsl_t)) :=
   let owner := int64_to_pid tsl.(types_tsl_t_owner) in
   let free := int64_to_nat tsl.(types_tsl_t_cfree) in
@@ -41,32 +55,33 @@ Definition tsl_up (tsl : Types_tsl_t) : option (option (cap_t tsl_t)) :=
   mk_cap_opt owner free size data.
 
 Definition mon_up (mon : Types_mon_t) : option (option (cap_t mon_t)) :=
-  match int64_to_pid mon.(types_mon_t_pid) with
-  | None => None
-  | Some pid =>
-    let owner := int64_to_pid mon.(types_mon_t_owner) in
-    let free := int64_to_nat mon.(types_mon_t_cfree) in
-    let size := int64_to_nat mon.(types_mon_t_csize) in
-    let data := {| mpid := pid; |} in
-    mk_cap_opt owner free size data
-  end.
+  pid ← int64_to_pid mon.(types_mon_t_pid);
+  let owner := int64_to_pid mon.(types_mon_t_owner) in
+  let free := int64_to_nat mon.(types_mon_t_cfree) in
+  let size := int64_to_nat mon.(types_mon_t_csize) in
+  let data := {| mpid := pid; |} in
+  mk_cap_opt owner free size data.
 
-Definition tsl_table_up l :=
-  match mmap tsl_up l with
-  | None => None
-  | Some tsl_table => Some (CapTable tsl_table)
-  end.
+(** Mappings from concrete capability table to abstract capability table.
+Using stdpp list monad operation [mapM]:
+   https://plv.mpi-sws.org/coqdoc/stdpp/stdpp.list_monad.html *)
+Definition tsl_table_up (l : list Types_tsl_t) : option tsl_table_t :=
+  tsl_table ← mapM tsl_up l; mret (CapTable tsl_table).
 
-Definition mon_table_up (l : list Types_mon_t) :=
-  match mmap mon_up l with
-  | None => None
-  | Some mon_table => Some (CapTable mon_table)
-  end.
+Definition mon_table_up (l : list Types_mon_t) : option mon_table_t :=
+  mon_table ← mapM mon_up l; mret (CapTable mon_table).
+
+(* TODO complete refinement mappings *)
+Parameter mem_up : Types_mem_t -> mem_t.
+
+Definition mem_table_up := map mem_up.
+Parameter some_mem_table : mem_table_t.
+
+
+(** Process control block  mappings. *)
 Parameter regs_up : list int64 -> regs_t.
-
 Parameter pmp_up : Types_pmp_t -> pmp_t.
-
-(* psuspend or busy flag *)
+(** psuspend and busy flag *)
 Parameter pstate_to_flags : int64 -> (bool * bool).
 
 Definition proc_up (p : Types_proc_t) : proc_t :=
@@ -75,46 +90,30 @@ Definition proc_up (p : Types_proc_t) : proc_t :=
      psuspend := fst (pstate_to_flags p.(types_proc_t_state)); |}.
 
 Definition ptable_up := map proc_up.
-Parameter mem_up : Types_mem_t -> mem_t.
 
-Definition mem_table_up := map mem_up.
-
+(** Scheduler mappings. *)
 Parameter some_sched : sched_t.
 
-Parameter some_mem_table : mem_table_t.
-
-(* TODO maybe we should use some option monad notation *)
-(* Alternatively, can define a version of kstate_to_kstate that is total. *)
-Definition kstate_to_kstate (k : Types_kstate) : option kstate_t :=
-  match mon_table_up k.(types_kstate_mon_table) with
-  | None => None
-  | Some mon_table =>
-      match tsl_table_up k.(types_kstate_tsl_table) with
-      | None => None
-      | Some tsl_table =>
-        Some {|
-          kptable := ptable_up k.(types_kstate_procs);
-          ktsl_tbl := tsl_table;
-          kmon_tbl := mon_table;
-          kmem_tbl := some_mem_table;
-          ksched := some_sched;
-        |}
-      end
-  end.
+Definition kstate_up (k : Types_kstate) : option kstate_t :=
+  mon_table ← mon_table_up k.(types_kstate_mon_table);
+  tsl_table ← tsl_table_up k.(types_kstate_tsl_table);
+  mret {|
+    kptable := ptable_up k.(types_kstate_procs);
+    ktsl_tbl := tsl_table;
+    kmon_tbl := mon_table;
+    kmem_tbl := some_mem_table;
+    ksched := some_sched;
+  |}.
 
 Definition kstate_to_kstate_err (k : Types_kstate) : option (kstate_t * int64) :=
-  match kstate_to_kstate k with
-  | None => None
-  | Some k' => Some (k', k.(types_kstate_errcode))
-  end.
+  k' ← kstate_up k; mret (k', k.(types_kstate_errcode)).
 
+(** Relational version of refinement mappings. *)
 Definition Rnat : nat -> int64 -> Prop := fun_hrel int64_to_nat.
-
-Definition Rnat_usz : nat -> usize -> Prop := fun_hrel usize_to_nat.
 
 Definition Rpid : nat -> int64 -> Prop := ofun_hrel int64_to_pid.
 
-Definition Rpid_opt := fun_hrel int64_to_pid.
+Definition Rpid_opt : option nat -> int64 -> Prop := fun_hrel int64_to_pid.
 
 Definition Rtsl := ofun_hrel tsl_up.
 
@@ -130,32 +129,223 @@ Parameter kstate_to_ctx : Types_kstate -> ctx_t.
 
 Definition Rctx := fun_hrel kstate_to_ctx.
 
-Definition Rkstate := ofun_hrel kstate_to_kstate.
+Definition Rkstate := ofun_hrel kstate_up.
 
 Definition Rkstate_with_err := ofun_hrel kstate_to_kstate_err.
 
-Lemma Rkstate_equiv :
+Create HintDb s3k_repr_unfold.
+Hint Unfold mbind option_bind : s3k_repr_unfold.
+Hint Unfold fun_hrel ofun_hrel : s3k_repr_unfold.
+Hint Unfold kstate_up kstate_to_kstate_err : s3k_repr_unfold.
+Hint Unfold Rtsl_table Rmon_table Rptable Rctx Rkstate Rkstate_with_err : s3k_repr_unfold.
+
+(** ** Helper lemmas *)
+
+(** Lemmas used for backward reasoning. *)
+(* FIXME this is ignoring memory table and scheduler for now. *)
+Lemma Rkstate_inv :
   forall ka kb,
-  Rkstate ka kb <->
-  Rmon_table ka.(kmon_tbl) kb.(types_kstate_mon_table) /\
-    Rtsl_table ka.(ktsl_tbl) kb.(types_kstate_tsl_table) /\
-    Rptable ka.(kptable) kb.(types_kstate_procs).
+  (Rmon_table ka.(kmon_tbl) kb.(types_kstate_mon_table) /\
+   Rtsl_table ka.(ktsl_tbl) kb.(types_kstate_tsl_table) /\
+   Rptable ka.(kptable) kb.(types_kstate_procs)) ->
+  Rkstate ka kb.
 Proof.
+  autounfold with s3k_repr_unfold.
+  intros.
+  unfold kstate_up.
+  destruct_and?.
+  rewrite H0, H2, H.
 Admitted.
 
-Lemma Rkstate_with_err_equiv :
+Lemma Rmon_table_inv_Rkstate :
+  forall ka kb, Rkstate ka kb ->
+  Rmon_table ka.(kmon_tbl) kb.(types_kstate_mon_table).
+Proof.
+  autounfold with s3k_repr_unfold.
+  intros; repeat case_match; try discriminate; by inv H.
+Qed.
+
+Lemma Rtsl_table_inv_Rkstate :
+  forall ka kb, Rkstate ka kb ->
+  Rtsl_table ka.(ktsl_tbl) kb.(types_kstate_tsl_table).
+Proof.
+  autounfold with s3k_repr_unfold.
+  intros; repeat case_match; try discriminate; by inv H.
+Qed.
+
+Lemma Rptable_inv_Rkstate :
+  forall ka kb, Rkstate ka kb ->
+  Rptable ka.(kptable) kb.(types_kstate_procs).
+Proof.
+  autounfold with s3k_repr_unfold.
+  intros; repeat case_match; try discriminate; by inv H.
+Qed.
+
+Lemma Rkstate_with_err_inv :
   forall ka kb erra,
-  Rkstate_with_err (ka, erra) kb <->
-  Rkstate ka kb /\ erra = kb.(types_kstate_errcode).
+  (Rkstate ka kb /\ erra = kb.(types_kstate_errcode)) ->
+  Rkstate_with_err (ka, erra) kb.
 Proof.
-Admitted.
+  unfold Rkstate_with_err, Rkstate, kstate_to_kstate_err, fun_hrel, ofun_hrel.
+  intros.
+  destruct H.
+  by rewrite H, H0.
+Qed.
 
-Lemma Rmon_equiv :
+
+Local Transparent Archi.ptr64 Wordsize_Ptrofs.wordsize.
+
+Lemma int64_to_usize_to_nat_same ia ib:
+  Rnat ia ib ->
+  usize_to_nat (USIZE.of_u64 ib) = ia.
+Proof.
+  unfold Rnat, fun_hrel.
+  intros.
+  rewrite <- H.
+  unfold usize_to_nat, int64_to_nat, USIZE.to_Z, USIZE.of_u64.
+  f_equal.
+  apply Ptrofs.unsigned_repr.
+  replace Ptrofs.max_unsigned with Int64.max_unsigned by reflexivity.
+  apply Int64.unsigned_range_2.
+Qed.
+
+Lemma Rmon_table_set :
+  forall ta tb ia (ib : int64) va vb tb',
+  tb.[ib <- vb] = Some tb' ->
+  Rmon_table ta tb ->
+  Rmon va vb ->
+  Rnat ia ib ->
+  Rmon_table (cap_set ta (ia, va)) tb'.
+Proof.
+  autounfold with s3k_repr_unfold.
+  intros.
+  unfold mon_table_up, mbind in *.
+  (* Avoid unfolding the implicit argument to mapM. *)
+  unfold option_bind at 1.
+  unfold option_bind in H0.
+  case_match; try discriminate.
+  apply mapM_Some_1 in H3.
+  unfold Rmon, ofun_hrel in H1.
+  pose proof Forall2_insert _ _ _ _ _ ia H3 H1.
+  rewrite (bset_Some_insert tb ib vb H).
+  rewrite (int64_to_usize_to_nat_same H2).
+  unfold cap_set.
+  inv H0.
+  apply mapM_Some_2 in H4.
+  by rewrite H4.
+Qed.
+
+Lemma Rmon_set_owner :
+  forall mona monb ownera ownerb,
+  Rmon (Some mona) monb ->
+  Rpid_opt ownera ownerb ->
+  let monb' := monb <| types_mon_t_owner := ownerb |> in
+  let mona' := mona <| (@cowner mon_t) := ownera |> in
+  Rmon (Some mona') monb'.
+Proof.
+  unfold Rmon, ofun_hrel, mon_up, mbind, option_bind, mk_cap_opt.
+  intros.
+  case_match; try discriminate. 
+  unfold Rpid_opt, fun_hrel in H0.
+  repeat case_match; try discriminate; simpl in *. 
+  - lia.
+  - lia.
+  - inv H. f_equal. f_equal. simpl. congruence.
+  - congruence.
+Qed.
+
+(** Lemmas used for forward reasoning *)
+
+Lemma Rmon_Some_corres :
   forall va vb,
   Rmon (Some va) vb ->
-  Rnat va.(cfree) vb.(types_mon_t_cfree) /\
+  Rpid_opt va.(cowner) vb.(types_mon_t_owner) /\
+    Rnat va.(cfree) vb.(types_mon_t_cfree) /\
     Rnat va.(csize) vb.(types_mon_t_csize) /\
-    Rpid_opt va.(cowner) vb.(types_mon_t_owner).
+    Rpid_opt (Some va.(cdata).(mpid)) vb.(types_mon_t_pid).
+Proof.
+  intros.
+  unfold Rmon, ofun_hrel, mon_up, mbind, option_bind, mk_cap_opt in H.
+  repeat case_match; try discriminate.
+  inv H.
+  by repeat split.
+Qed.
+
+Lemma mon_get_Some_corres :
+  forall ta tb ia ib va,
+  Rmon_table (CapTable ta) tb ->
+  Rnat ia ib ->
+  ta !! ia = Some va ->
+  exists vb, tb.[ib] = Some vb /\ Rmon va vb.
+Proof.
+  intros.
+  unfold Rmon_table, ofun_hrel, mon_table_up, mbind, option_bind in H.
+  case_match; try discriminate.
+  inv H.
+  apply mapM_Some in H2.
+  pose proof Forall2_length _ _ _ H2.
+  pose proof lookup_lt_Some _ _ _ H1.
+  rewrite bget_lookup.
+  rewrite (int64_to_usize_to_nat_same H0).
+  rewrite <- H in H3.
+  apply lookup_lt_is_Some in H3.
+  destruct H3.
+  eexists x.
+  split.
+  - done.
+  - by pose proof Forall2_lookup_lr _ _ _ _ _ _ H2 H3 H1.
+Qed.
+
+Lemma Rmon_None_corres :
+  forall ownera ownerb cb,
+  Rpid_opt (Some ownera) ownerb ->
+  Rmon None cb ->
+  Int64.eq cb.(types_mon_t_owner) ownerb = false.
+Proof.
+  unfold Rpid_opt, Rmon, mon_up, int64_to_pid, fun_hrel, ofun_hrel, mbind, option_bind, mk_cap_opt.
+  intros.
+  repeat case_match; try discriminate.
+  inv H.
+  norm_cmp in *.
+  congruence.
+Qed.
+
+Lemma Rpid_opt_inj ownera ownerb ownera' ownerb':
+  Rpid_opt ownera ownerb ->
+  Rpid_opt ownera' ownerb' ->
+  (ownera = ownera' <-> Int64.unsigned ownerb = Int64.unsigned ownerb').
+Proof.
+  unfold Rpid_opt, fun_hrel, mon_up, int64_to_pid.
+  intros.
+  repeat case_match; try discriminate.
+  all: norm_cmp in *; subst; try (split; congruence).
+  unfold int64_to_nat.
+  repr_elim in *.
+  split; intros.
+  - inv H. rep_lia.
+  - f_equal. rep_lia.
+Qed.
+
+Section Length.
+
+Variable ta : list (option (cap_t mon_t)).
+Hypothesis mon_table_size : ctable_size (CapTable ta) = MON_SZ.
+  
+Lemma mon_lookup_Some_len :
+  forall ia ib va,
+  ta !! ia = Some va ->
+  Rnat ia ib ->
+  Int64.ltu ib Config_mon_table_size = true.
+Proof.
+  (* Use axioms about array lengths from invariants.v *)
+Admitted.
+
+Lemma mon_lookup_None_len :
+  forall ia ib,
+  ta !! ia = None ->
+  Rnat ia ib ->
+  Int64.ltu ib Config_mon_table_size = false.
 Proof.
 Admitted.
 
+End Length.
