theories/Verif/barocq_aux.v
@@ -1,0 +1,96 @@
+From stdpp Require Import prelude.
+From compcert Require Import Integers.
+From S3K.BarocqComp Require Import Intop Barray.
+From S3K.BarocqComp Require Import ShallowNotations.
+From S3K.Verif Require Import tactics.
+From VST Require Import Zlist.
+
+Set Implicit Arguments.
+
+(** * Barray helper lemmas  *)
+
+(** Usize integer (architecture specific) to natural number. *)
+Definition usize_to_nat (i : usize) : nat := Z.to_nat (USIZE.to_Z i).
+
+Section Barray.
+
+Variable A : Type.
+
+Lemma bget_lookup :
+  forall (t : list A) i, t.[i] = t !! (usize_to_nat i).
+Proof.
+  intros.
+  unfold get, usize_to_nat, USIZE.to_Z.
+  set (z := Intsize.unsigned i).
+  assert (0 <= z) by rep_lia.
+  rewrite <- (Z2Nat.id z H).
+  rewrite Nat2Z.id.
+  generalize (Z.to_nat z) as n.
+  clear z H.
+  revert t.
+  induction t.
+  - reflexivity.
+  - destruct n.
+    + reflexivity.
+    + simpl; rewrite <- Nat2Z.inj_pred; [ done | by lia ].
+Qed.
+
+Lemma valid_index_true_length (t : list A) i :
+  valid_index t i = true -> (usize_to_nat i < length t)%nat.
+Proof.
+  intros.
+  unfold valid_index in H.
+  apply Z.ltb_lt in H.
+  change Barray.Zlength with Zlength in H.
+  rewrite <- ZtoNat_Zlength.
+  unfold usize_to_nat, USIZE.to_Z.
+  rep_lia.
+Qed.
+
+Lemma bget_Some :
+  forall (t : list A) i,
+  t.[i] <> None <-> (usize_to_nat i < length t)%nat.
+Proof.
+  intros.
+  unfold get, usize_to_nat, USIZE.to_Z.
+  set (z := Intsize.unsigned i) in *.
+  assert (0 <= z) by rep_lia.
+  rewrite ZlistPlus.list_nth_z_Some.
+  rewrite <- ZtoNat_Zlength.
+  lia.
+Qed.
+
+(** TODO this one is tricky *)
+Lemma bset_Some_insert :
+  forall (t t' : list A) i v,
+  t.[i <- v] = Some t' ->
+  t' = <[ usize_to_nat i := v ]> t.
+Proof.
+  (* setSPEC is insufficient for this proof since it only specifies
+     indices within the usize range are unchanged. *)
+  intros.
+  unfold set in H; case_match; try discriminate.
+  pose proof valid_index_true_length _ _ H0.
+  inv H.
+  unfold usize_to_nat, USIZE.to_Z in *.
+  set (z := Intsize.unsigned i) in *.
+  assert (0 <= z) by rep_lia.
+  rewrite <- (Z2Nat.id z H).
+  rewrite Nat2Z.id.
+  set (n := Z.to_nat z) in *.
+  apply list_eq.
+  intros n'.
+  assert (n' < n \/ n' = n \/ n < n')%nat by lia.
+  destruct_or?.
+  - (* n' < n *)
+Admitted.
+
+Lemma bget_Some_bset_Some :
+  forall (t : list A) i v v',
+  t.[i] = Some v ->
+  exists t', t.[i <- v'] = Some t'.
+Proof.
+Admitted.
+
+End Barray.
+
