theories/Verif/invariants.v
@@ -1,0 +1,26 @@
+From S3K.Barocq Require Import S3K_ShallowR.
+From S3K.ExecSem Require Import util config.
+
+(** * Invariants and axioms *)
+
+Section ExecSem.
+
+(** Specify absract kernel configurations with concrete numbers. *)
+Axiom proc_cnt_config : PROC_CNT = int64_to_nat Config_max_pid.
+Axiom hart_cnt_config : HART_CNT = int64_to_nat Platform_num_harts .
+Axiom mon_sz_config : MON_SZ = int64_to_nat Config_mon_table_size.
+Axiom tsl_sz_config : TSL_SZ = int64_to_nat Config_tsl_table_size.
+
+End ExecSem.
+
+Section Barocq.
+
+Variable kb : Types_kstate.
+
+(** Array Barocq kernel state should have fixed lengths given at compile time. *)
+Axiom kb_tsl_len : length kb.(types_kstate_tsl_table) = int64_to_nat Config_tsl_table_size.
+Axiom kb_mon_len : length kb.(types_kstate_mon_table) = int64_to_nat Config_mon_table_size.
+Axiom kb_procs_len : length kb.(types_kstate_procs) = int64_to_nat Config_max_pid.
+
+End Barocq.
+
