theories/Verif/tactics.v
@@ -1,0 +1,152 @@
+From stdpp Require Import prelude.
+From compcert Require Import Coqlib Integers.
+
+(** * Tactics *)
+
+(** Normalize Int64 comparisons into Z comparisons *)
+Lemma ltu_true :
+  forall x y, Int64.ltu x y = true <-> (Int64.unsigned x) < (Int64.unsigned y).
+Proof.
+  split; intros.
+  - unfold Int64.ltu in H. destruct zlt in H; [ assumption | discriminate ].
+  - unfold Int64.ltu. destruct zlt; [ reflexivity | contradiction ].
+Qed.
+
+Lemma ltu_false :
+  forall x y, Int64.ltu x y = false  <-> (Int64.unsigned x) >= (Int64.unsigned y).
+Proof.
+  split; intros.
+  - unfold Int64.ltu in H. destruct zlt in H; [ discriminate | assumption ].
+  - unfold Int64.ltu. destruct zlt; [ contradiction | reflexivity ].
+Qed.
+
+Lemma eq_true :
+  forall x y, Int64.eq x y = true <-> (Int64.unsigned x) = (Int64.unsigned y).
+Proof.
+  split; intros.
+  - unfold Int64.eq in H. destruct zeq in H; [ assumption | discriminate ].
+  - unfold Int64.eq. destruct zeq; [ reflexivity | contradiction ].
+Qed.
+
+Lemma eq_false :
+  forall x y, Int64.eq x y = false <-> (Int64.unsigned x) <> (Int64.unsigned y).
+Proof.
+  split; intros.
+  - unfold Int64.eq in H. destruct zeq in H; [ discriminate | assumption ].
+  - unfold Int64.eq. destruct zeq; [ contradiction | reflexivity ].
+Qed.
+
+Ltac norm_cmp :=
+  unfold Int64.cmpu, Int64.cmp;
+  repeat rewrite ?negb_true_iff, ?negb_false_iff;
+  repeat rewrite ?eq_true, ?eq_false, ?ltu_true, ?ltu_false.
+
+Tactic Notation "norm_cmp" "in" hyp(H) :=
+  unfold Int64.cmpu, Int64.cmp in H;
+  repeat rewrite ?negb_true_iff, ?negb_false_iff in H;
+  repeat rewrite ?eq_true, ?eq_false, ?ltu_true, ?ltu_false in H.
+
+Tactic Notation "norm_cmp" "in" "*" :=
+  repeat_on_hyps (fun H => norm_cmp in H); norm_cmp.
+
+(** rep_lia from VST *)
+
+Ltac Zground X :=
+  match X with
+  | Z0 => idtac
+  | Zpos ?y => Zground y
+  | Zneg ?y => Zground y 
+  | xH => idtac
+  | xO ?y => Zground y
+  | xI ?y => Zground y
+ end.
+
+Ltac pose_const_equation X :=
+ match goal with
+ | H: X = ?Y |- _ => Zground Y
+ | _ => let z := eval compute in X in 
+            match z with context C [Archi.ptr64] =>
+                       first [
+                           unify Archi.ptr64 false; let u := context C [false] in let u := eval compute in u in change X with u in *
+                          |unify Archi.ptr64 true; let u := context C [true] in let u := eval compute in u in change X with u in *
+                      ]
+              | _ => change X with z in *
+            end
+ end.
+
+Ltac perhaps_post_const_equation X :=
+ lazymatch goal with 
+ | H: context [X] |- _ => pose_const_equation X
+(* | H:= context [X] |- _ => pose_const_equation X *)
+ | |- context [X] => pose_const_equation X
+ | |- _ => idtac
+ end.
+
+Ltac pose_const_equations L :=
+ match L with
+ | ?X :: ?Y => perhaps_post_const_equation X; pose_const_equations Y
+ | nil => idtac
+ end.
+
+Import ListNotations.
+
+Ltac pose_standard_const_equations :=
+pose_const_equations
+  [
+  Int.zwordsize; Int.modulus; Int.half_modulus; Int.max_unsigned; Int.max_signed; Int.min_signed;
+  Int64.zwordsize; Int64.modulus; Int64.half_modulus; Int64.max_unsigned; Int64.max_signed; Int64.min_signed;
+  Ptrofs.zwordsize; Ptrofs.modulus; Ptrofs.half_modulus; Ptrofs.max_unsigned; Ptrofs.max_signed; Ptrofs.min_signed;
+  Byte.min_signed; Byte.max_signed; Byte.max_unsigned; Byte.modulus
+  ];
+ pose_const_equations [Int.wordsize; Int64.wordsize; Ptrofs.wordsize].
+
+Ltac pose_lemma F A L :=
+  match type of (L A) with ?T =>
+     lazymatch goal with
+      | H:  T |- _ => fail
+      | H:  T /\ _ |- _ => fail
+      | |- _ => pose proof (L A)
+     end
+  end.
+
+Ltac pose_lemmas F L :=
+ repeat
+  match goal with
+  | |- context [F ?A] => pose_lemma F A L
+  | H: context [F ?A] |- _ => pose_lemma F A L
+ end.
+
+Ltac rep_lia_setup := 
+ repeat match goal with
+            | x := _ : ?T |- _ => lazymatch T with Z => fail | nat => fail | _ => clearbody x end
+            end;
+ zify;
+  try autorewrite with rep_lia in *;
+  try autounfold with rep_lia in *;
+  pose_lemmas Byte.unsigned Byte.unsigned_range;
+  pose_lemmas Byte.signed Byte.signed_range;
+  pose_lemmas Int.unsigned Int.unsigned_range;
+  pose_lemmas Int.signed Int.signed_range;
+  pose_lemmas Int64.unsigned Int64.unsigned_range;
+  pose_lemmas Int64.signed Int64.signed_range;
+  pose_lemmas Ptrofs.unsigned Ptrofs.unsigned_range;
+  pose_standard_const_equations.
+
+Ltac rep_lia_setup2 := idtac.
+
+Ltac rep_lia :=
+   rep_lia_setup;
+   rep_lia_setup2;
+   lia.
+
+(** Rewrite Int64.unsigned (Int64.repr z) into z *)
+
+Ltac repr_elim :=
+  rewrite ?Int64.unsigned_repr by rep_lia.
+
+Tactic Notation "repr_elim" "in" hyp(H) :=
+  rewrite ?Int64.unsigned_repr in H by rep_lia.
+
+Tactic Notation "repr_elim" "in" "*" :=
+  repeat_on_hyps (fun H => repr_elim in H); repr_elim.
+
